Logic/Predicate/FirstOrder/Arith/Model.lean
@@ -1,0 +1,36 @@
+import Logic.Predicate.FirstOrder.Semantics
+
+namespace FirstOrder
+
+namespace Arith
+open Language
+
+namespace Semantics
+
+instance StandardModel : Structure oring ℕ where
+  func := fun f =>
+    match f with
+    | ORingFunc.zero => fun _ => 0
+    | ORingFunc.one  => fun _ => 1
+    | ORingFunc.add  => fun v => v 0 + v 1
+    | ORingFunc.mul  => fun v => v 0 * v 1
+  rel := fun r =>
+    match r with
+    | ORingRel.eq => fun v => v 0 = v 1
+    | ORingRel.lt => fun v => v 0 < v 1
+
+variable (L : Language.{u}) [L.ORing]
+
+structure Cut (M : Type w) [s : Structure L M] where
+  domain : Set M
+  closedSucc : ∀ x ∈ domain, (ᵀ“#0 + 1”).bVal s ![x] ∈ domain
+  closedLt : ∀ x y : M, SubFormula.BVal s ![x, y] “#0 < #1” → y ∈ domain → x ∈ domain
+
+structure ClosedCut (M : Type w) [s : Structure L M] extends Structure.ClosedSubset L M where
+  closedLt : ∀ x y : M, SubFormula.BVal s ![x, y] “#0 < #1” → y ∈ domain → x ∈ domain
+
+end Semantics
+
+end Arith
+
+end FirstOrder
